Updates.

ClassicalLogicLean/NV/Fresh.lean
@@ -4,86 +4,92 @@ import Mathlib.Tactic
 import Mathlib.Data.String.Lemmas
 
 
-set_option autoImplicit false
+set_option linter.style.docString false
+set_option linter.style.emptyLine false
+set_option linter.style.longLine false
 
 
 /--
-  `finset_var_name_max_len xs` := The length of the longest variable name in the finite set of variable names `xs` or 0 if the set is empty.
+  `finset_var_name_max_len css` := The length of the longest variable name in the finite set of variable names `css` or 0 if the set is empty.
 -/
 def finset_var_name_max_len :
   Finset VarName_ → ℕ :=
   Finset.fold (fun (m n : ℕ) => max m n) 0 (fun (x : VarName_) => x.length)
 
 
-lemma finset_var_name_max_len_mem
-  (x : VarName_)
-  (xs : Finset VarName_)
-  (h1 : x ∈ xs) :
-  x.length ≤ finset_var_name_max_len xs :=
+theorem finset_var_name_max_len_mem
+  (cs : VarName_)
+  (css : Finset VarName_)
+  (h1 : cs ∈ css) :
+  cs.length ≤ finset_var_name_max_len css :=
   by
-  induction xs using Finset.induction_on
-  case empty =>
-    simp at h1
-  case insert hd tl a1 ih =>
-    simp at h1
+    induction css using Finset.induction_on
+    case empty =>
+      simp only [Finset.notMem_empty] at h1
+    case insert hd tl ih_1 ih_2 =>
+      simp only [Finset.mem_insert] at h1
 
-    cases h1
-    case inl c1 =>
-      subst c1
-      simp only [finset_var_name_max_len]
-      simp
-    case inr c1 =>
-      simp only [finset_var_name_max_len] at ih
+      cases h1
+      case inl h1 =>
+        rewrite [h1]
+        unfold finset_var_name_max_len
+        simp only [Finset.fold_insert_idem, le_sup_left]
+      case inr h1 =>
+        simp only [finset_var_name_max_len] at ih_2
 
-      simp only [finset_var_name_max_len]
-      simp
-      right
-      exact ih c1
+        simp only [finset_var_name_max_len]
+        simp only [Finset.fold_insert_idem, le_sup_iff]
+        right
+        apply ih_2
+        exact h1
 
 
 /--
-  `fresh x c xs` := If the variable name `x` is not a member of the finite set of variable names `xs` then `x` is returned. If `x` is a member of `xs` then the character `c` is repeatedly appended to `x` until the resulting variable name is not a member of `xs`. The resulting variable name is then returned.
+  `fresh cs c css` := If the variable name `cs` is not a member of the finite set of variable names `css` then `cs` is returned. If `cs` is a member of `css` then the character `c` is repeatedly appended to `cs` until the resulting variable name is not a member of `css`. The resulting variable name is then returned.
 -/
 def fresh
-  (x : VarName_)
+  (cs : VarName_)
   (c : Char)
-  (xs : Finset VarName_) :
+  (css : Finset VarName_) :
   VarName_ :=
-  if h : x ∈ xs
+  if h : cs ∈ css
   then
-    have : finset_var_name_max_len xs - x.length < finset_var_name_max_len xs + 1 - x.length :=
+    have : (finset_var_name_max_len css) - cs.length < (finset_var_name_max_len css) + 1 - cs.length :=
     by
       apply Nat.sub_lt_sub_right
       · apply finset_var_name_max_len_mem
         exact h
       · apply lt_add_one
-  fresh (VarName_.mk (x.toString ++ c.toString)) c xs
-  else x
-  termination_by finset_var_name_max_len xs + 1 - x.length
+  fresh (VarName_.mk (cs.toString ++ c.toString)) c css
+  else cs
+  termination_by (finset_var_name_max_len css) + 1 - cs.length
 
 
-lemma fresh_not_mem
-  (x : VarName_)
+theorem fresh_not_mem
+  (cs : VarName_)
   (c : Char)
-  (xs : Finset VarName_) :
-  fresh x c xs ∉ xs :=
-  if h : x ∈ xs
+  (css : Finset VarName_) :
+  fresh cs c css ∉ css :=
+  if h : cs ∈ css
   then
-  have : finset_var_name_max_len xs - x.length < finset_var_name_max_len xs + 1 - x.length :=
-  by
-    apply Nat.sub_lt_sub_right
-    · apply finset_var_name_max_len_mem
-      exact h
-    · apply lt_add_one
+    have : (finset_var_name_max_len css) - cs.length < (finset_var_name_max_len css) + 1 - cs.length :=
+    by
+      apply Nat.sub_lt_sub_right
+      · apply finset_var_name_max_len_mem
+        exact h
+      · apply lt_add_one
   by
     unfold fresh
-    split_ifs
-    apply fresh_not_mem
+    split
+    case isTrue c1 =>
+      apply fresh_not_mem
+    case isFalse c1 =>
+      contradiction
   else by
     unfold fresh
-    split_ifs
-    exact h
-  termination_by finset_var_name_max_len xs + 1 - x.length
-
-
-#lint
+    split
+    case isTrue c1 =>
+      contradiction
+    case isFalse c1 =>
+      exact h
+  termination_by (finset_var_name_max_len css) + 1 - cs.length
