ClassicalLogicLean/NV/Parse.lean
@@ -3,7 +3,9 @@ import Lean
 import ClassicalLogicLean.NV.Formula
 
 
-set_option autoImplicit false
+set_option linter.style.docString false
+set_option linter.style.emptyLine false
+set_option linter.style.longLine false
 
 
 open Formula_
